Progress on PROB effect

Probabilism.fst
@@ -2,40 +2,90 @@ module Probabilism
 
 open FStar.Real
 
-type pr = p:real{p >=. 0.0R}
-type prob_post a = a -> GTot pr
-type prob_pre = pr
-type prob_wp a = prob_post a -> GTot prob_pre
+let pr = p:real{p >=. 0.0R}
+let prob_post (a:Type) = a -> Tot pr
+let prob_pre = pr
+let prob_wp (a:Type) = prob_post a -> Tot prob_pre
 
-assume val distribution : (a:Type) -> Type
+(*noeq
+type distribution (a:Type) : Type =
+    | Point : a -> distribution a
+    | Bind : b:Type -> distribution b -> (b -> distribution a) -> distribution a
+    *)
 
-assume val point_distribution : (a:Type) -> a -> distribution a
+assume type distribution (a:Type) : Type
 
-type prob (a:Type) (w:prob_wp a): Type =
+assume val point_distribution (#a:Type) (x:a) : distribution a
+
+let prob (a:Type) (w:prob_wp a): Tot Type0 =
   distribution a // TODO: require w to hold
 
 let prob_wreturn a x : prob_wp a = fun(p:prob_post a) -> p x
 
 let prob_return a (x:a) : prob a (prob_wreturn a x) = 
-  point_distribution a x
+  point_distribution x
 
 let prob_wbind a b (w1:prob_wp a) (w2:a -> prob_wp b) : prob_wp b = fun p -> w1 (fun x -> w2 x p)
 
 let prob_bind a b (w1:prob_wp a) (w2:a -> prob_wp b)
-      (f: prob a w1) (g: (x:a -> prob b (w2 x))) : prob b (prob_wbind a b w1 w2) = 
-  admit()
+      (f: prob a w1) (g: (x:a -> prob b (w2 x))) : prob b (prob_wbind a b w1 w2) =
+   admit()   
 
-reifiable reflectable new_effect { PROB : (a:Type) -> Effect with 
+reflectable
+layered_effect { PROB : (a:Type) -> (wp:prob_wp a) -> Effect with 
   repr = prob;
   return = prob_return; 
   bind = prob_bind
-(*  if_then_else = admit();
-  ite_wp = admit();
-  stronger = admit();
-  close_wp = admit();
-  assert_p = admit();
-  assume_p = admit();
-  null_wp = admit();
-  trivial = admit() *)
   }
-  
+
+//let ret (#a) (x:a) : PROB a (fun post -> post x) =
+//    PROB?.reflect (prob_return a x)
+
+// let test () : PROB string (fun post -> post "hello") = 
+//    PROB?.reflect (prob_return string "hello")
+
+    
+assume val largest : (pr -> Tot Type0) -> Tot pr
+
+let lemmaxxx () : Lemma(forall post.
+largest (fun r -> (fun p -> p "hello") (fun x -> post x >=. r))
+=
+post "hello"
+)
+= admit()
+
+let lift_pure_prob_wp (a:Type) (wp:pure_wp a) : prob_wp a = 
+    // TODO
+    (fun post -> largest (fun r -> wp (fun x -> post x >=. r)))
+//admit()
+
+
+let hellemma : 
+squash(forall (ppost: (_: string -> pr)) (x: string).
+  (forall (post: (_: string -> Type0)).
+     (forall (return_val: string). return_val == "hello" ==> post return_val) ==> post x) ==>
+     ppost "hello" = ppost x)
+= admit()
+
+let compatible (#a) (wp:pure_wp a) (pwp:prob_wp a) = 
+    forall ppost x.
+       (forall post. wp post ==> post x) ==> pwp ppost = (* TODO <= *) ppost x
+
+let lift_pure_prob (a:Type) (#pwp:prob_wp a) (wp:pure_wp a) (f: eqtype_as_type unit -> PURE a wp) : 
+   Pure (prob a pwp) (requires compatible wp pwp) (fun x -> ensures True) =
+ //  largest (fun r -> wp (fun x -> p x >=. r))
+  admit()
+
+sub_effect PURE ~> PROB = lift_pure_prob
+
+(*
+assume val lem1: squash (
+       lift_pure_prob_wp string (fun p -> p "hello") == (fun p -> p "hello")
+)*)
+
+
+// let test3 () : PROB string (fun p -> p "hello") = "hello"
+
+// let test2 () : PROB string (fun post -> post "hello") = test ()
+
+// let reified = reify (test2 ())
